Use ch2o

main/Main.hs
@@ -7,57 +7,66 @@ import System.IO
 import Text.Parsec (parse)
 import Text.Parsec.Combinator (eof)
 
-import Ast
-import Entities (Coq_heap, Coq_frame, Coq_local_id(..), Coq_value(..))
-import Eval
-import Extract (init)
-import Parser (expr)
+import qualified Parser
+import Extracted (Expr(..), Expr_hole, Heap, Value(..), Local_id(..), Frame)
+import qualified Extracted
 
-deriving instance Show Coq_value
-deriving instance Show Coq_local_id
-deriving instance Eq Coq_local_id
-deriving instance Show Coq_expr
+deriving instance Show Value
+deriving instance Show Local_id
+deriving instance Show Expr
+deriving instance Show Expr_hole
+deriving instance Show (Extracted.Object)
+deriving instance Show (Extracted.N)
+deriving instance Show (Extracted.Positive)
+deriving instance (Show a) => Show (Extracted.Pmap_raw a)
+deriving instance (Show a) => Show (Extracted.Nmap a)
 
-type ST = (Coq_heap, Coq_frame)
+type ST = Heap
 type Repl = StateT ST (ExceptT String IO)
 
-gc :: Repl ()
-gc = modify gc'
-  where
-    gc' (heap, frame) = (heap, filter (isSourceId . fst) frame)
-    isSourceId (SourceId _) = True
-    isSourceId (TempId _) = False
+(init_heap, init_stack) = Extracted.init
 
-parser :: String -> Repl Coq_expr
-parser line = case parse (expr <* eof) "<interactive>" line of
-  Right e -> return e
-  Left err -> throwError (show err)
+parser :: String -> Repl Expr
+parser line =
+  case parse (Parser.expr <* eof) "<interactive>" line of
+    Right e -> return e
+    Left err -> throwError (show err)
+
+evaluate' :: Expr -> [Frame] -> Repl Value
+evaluate' expr@(Expr_temp temp) [frame] = do
+  let Just x = Extracted.lookup (Extracted.frame_lookup Extracted.localmap_lookup_temp) temp frame in return x
+
+evaluate' expr stack = do
+  heap <- get
+
+  case Extracted.eval heap stack expr of
+    Just ((heap', stack'), expr') -> put heap' >> evaluate' expr' stack'
+    Nothing -> throwError "eval error"
+
+evaluate :: Expr -> Repl Value
+evaluate expr = evaluate' expr init_stack
 
 command :: String -> String -> Repl ()
-command "heap"  _ = gets fst >>= liftIO . print
-command "frame" _ = gets snd >>= liftIO . print
-command "clear" _ = put Extract.init
-command "gc" _ = gc
+command "heap"  _ = get >>= liftIO . print
+command "reset" _ = put init_heap
 command "parse" line = parser line >>= liftIO . print
 
 repl :: String -> Repl ()
+repl "" = return ()
 repl (':':line) =
   let (c, rest) = break isSpace line in
   command c (dropWhile isSpace rest)
 
 repl line = do
   e <- parser line
-  (heap, frame) <- get
-  let ((heap', frame'), temp) = eval heap frame e
-  case lookup (TempId temp) frame' of
-    Just Coq_v_null -> liftIO (putStrLn "null")
-    Just (Coq_v_addr addr) ->
-      let (Just object) = lookup addr heap'
+  value <- evaluate e
+  heap <- get
+
+  case value of
+    V_null -> liftIO (putStrLn "null")
+    V_addr addr ->
+      let (Just object) = Extracted.lookup Extracted.nlookup addr heap
       in liftIO (print object)
-
-  put (heap', frame')
-
-  gc
 
 replMany :: Repl ()
 replMany = forever $ do
@@ -67,7 +76,7 @@ replMany = forever $ do
 
 main :: IO ()
 main = do
-  result <- runExceptT (evalStateT replMany Extract.init)
+  result <- runExceptT (evalStateT replMany init_heap)
   case result of
     Left err -> putStrLn ("Fatal error:" ++ err)
     Right () -> return ()
