site_scons/site_tools/Coq.py
@@ -1,0 +1,1 @@
+../../ch2o/site_scons/site_tools/Coq.py
