src/Ast.v
@@ -1,30 +1,177 @@
 Require Import Coq.Strings.String.
 Require Import Coq.Lists.List.
+Require Import Coq.Numbers.BinNums.
 
 Inductive expr : Type :=
-| expr_temp : nat -> expr
+| expr_temp : N -> expr
 | expr_seq : expr -> expr -> expr
 | expr_recover : expr -> expr
 | expr_local : string -> expr
 | expr_assign_local : string -> expr -> expr
 | expr_field : expr -> string -> expr
 | expr_assign_field : expr -> string -> expr -> expr
+| expr_call : expr -> string -> expr
 .
 
-(*
-Inductive expr : Type :=
-| expr_this : expr
-| expr_var : string -> expr
-| expr_assign_var : string -> expr -> expr
-| expr_field : expr -> string -> expr
-| expr_assign_field : expr -> string -> expr -> expr
-| expr_call : expr -> string -> list expr -> expr
-
-| expr_seq : expr -> expr -> expr
-| expr_recover : expr -> expr
-| expr_null : expr
-| expr_term : nat -> expr
+Inductive expr_hole : Type :=
+| expr_hole_id : expr_hole
+| expr_hole_seq : expr_hole -> expr -> expr_hole
+| expr_hole_recover : expr_hole -> expr_hole
+| expr_hole_assign_local : string -> expr_hole -> expr_hole
+| expr_hole_field : expr_hole -> string -> expr_hole
+| expr_hole_assign_field1 : expr -> string -> expr_hole -> expr_hole
+| expr_hole_assign_field2 : expr_hole -> string -> N -> expr_hole
+| expr_hole_call1 : expr_hole -> string -> expr_hole
 .
+
+Inductive make_hole : expr -> expr -> expr_hole -> Prop :=
+| make_hole_id: forall e, make_hole e e expr_hole_id
+
+| make_hole_seq: forall e1 e2 eh e1', make_hole e1 eh e1' ->
+    make_hole (expr_seq e1 e2) eh (expr_hole_seq e1' e2)
+
+| make_hole_recover: forall e1 eh e1', make_hole e1 eh e1' ->
+    make_hole (expr_recover e1) eh (expr_hole_recover e1')
+
+| make_hole_assign_local: forall n e1 eh e1', make_hole e1 eh e1' ->
+    make_hole (expr_assign_local n e1) eh (expr_hole_assign_local n e1')
+
+| make_hole_field: forall e1 n eh e1', make_hole e1 eh e1' ->
+    make_hole (expr_field e1 n) eh (expr_hole_field e1' n)
+
+| make_hole_assign_field1: forall e1 n e2 eh e2', make_hole e2 eh e2' ->
+    make_hole (expr_assign_field e1 n e2) eh (expr_hole_assign_field1 e1 n e2')
+
+| make_hole_assign_field2: forall e1 n t eh e1', make_hole e1 eh e1' ->
+    make_hole (expr_assign_field e1 n (expr_temp t)) eh (expr_hole_assign_field2 e1' n t)
+
+| make_hole_call1: forall e1 n eh e1', make_hole e1 eh e1' ->
+    make_hole (expr_call e1 n) eh (expr_hole_call1 e1' n).
+
+Fixpoint fill_hole (cps: expr_hole) (filler: expr) : expr :=
+  match cps with
+  | expr_hole_id => filler
+  | expr_hole_seq cps' e2 => expr_seq (fill_hole cps' filler) e2
+  | expr_hole_recover cps' => expr_recover (fill_hole cps' filler)
+  | expr_hole_assign_local name cps' => expr_assign_local name (fill_hole cps' filler)
+  | expr_hole_field cps' name => expr_field (fill_hole cps' filler) name
+  | expr_hole_assign_field1 e1 name cps' => expr_assign_field e1 name (fill_hole cps' filler)
+  | expr_hole_assign_field2 cps' name t2 => expr_assign_field (fill_hole cps' filler) name (expr_temp t2)
+  | expr_hole_call1 cps' name => expr_call (fill_hole cps' filler) name
+  end.
+
+Fixpoint compose_hole (a: expr_hole) (b: expr_hole) : expr_hole :=
+  match a with
+  | expr_hole_id => b
+  | expr_hole_seq cps' e2 => expr_hole_seq (compose_hole cps' b) e2
+  | expr_hole_recover cps' => expr_hole_recover (compose_hole cps' b)
+  | expr_hole_assign_local name cps' => expr_hole_assign_local name (compose_hole cps' b)
+  | expr_hole_field cps' name => expr_hole_field (compose_hole cps' b) name
+  | expr_hole_assign_field1 e1 name cps' => expr_hole_assign_field1 e1 name (compose_hole cps' b)
+  | expr_hole_assign_field2 cps' name t2 => expr_hole_assign_field2 (compose_hole cps' b) name t2
+  | expr_hole_call1 cps' name => expr_hole_call1 (compose_hole cps' b) name
+  end.
+
+Require Import Coq.Program.Equality.
+
+Lemma id_fill: forall e, fill_hole expr_hole_id e = e.
+Proof. auto. Qed.
+
+Lemma id_compose_left: forall h1, compose_hole expr_hole_id h1 = h1.
+Proof. auto. Qed.
+
+Lemma id_compose_right: forall h1, compose_hole h1 expr_hole_id = h1.
+Proof.
+induction 0.
+auto.
+simpl. rewrite IHh1. reflexivity.
+simpl. rewrite IHh1. reflexivity.
+simpl. rewrite IHh1. reflexivity.
+simpl. rewrite IHh1. reflexivity.
+simpl. rewrite IHh1. reflexivity.
+simpl. rewrite IHh1. reflexivity.
+simpl. rewrite IHh1. reflexivity.
+Qed.
+
+Lemma composition: forall h1 h2 e,
+  fill_hole h2 (fill_hole h1 e) = fill_hole (compose_hole h2 h1) e.
+Proof.
+intros.
+dependent induction h1.
+rewrite id_compose_right.
+rewrite id_fill.
+reflexivity.
+
+dependent induction h2.
+rewrite id_fill. rewrite id_compose_left. reflexivity.
+simpl. rewrite <- IHh2. simpl. reflexivity.
+simpl. rewrite <- IHh2. simpl. reflexivity.
+simpl. rewrite <- IHh2. simpl. reflexivity.
+simpl. rewrite <- IHh2. simpl. reflexivity.
+simpl. rewrite <- IHh2. simpl. reflexivity.
+simpl. rewrite <- IHh2. simpl. reflexivity.
+simpl. rewrite <- IHh2. simpl. reflexivity.
+
+dependent induction h2.
+rewrite id_fill. rewrite id_compose_left. reflexivity.
+simpl. rewrite <- IHh2. simpl. reflexivity.
+simpl. rewrite <- IHh2. simpl. reflexivity.
+simpl. rewrite <- IHh2. simpl. reflexivity.
+simpl. rewrite <- IHh2. simpl. reflexivity.
+simpl. rewrite <- IHh2. simpl. reflexivity.
+simpl. rewrite <- IHh2. simpl. reflexivity.
+simpl. rewrite <- IHh2. simpl. reflexivity.
+
+dependent induction h2.
+rewrite id_fill. rewrite id_compose_left. reflexivity.
+simpl. rewrite <- IHh2. simpl. reflexivity.
+simpl. rewrite <- IHh2. simpl. reflexivity.
+simpl. rewrite <- IHh2. simpl. reflexivity.
+simpl. rewrite <- IHh2. simpl. reflexivity.
+simpl. rewrite <- IHh2. simpl. reflexivity.
+simpl. rewrite <- IHh2. simpl. reflexivity.
+simpl. rewrite <- IHh2. simpl. reflexivity.
+
+dependent induction h2.
+rewrite id_fill. rewrite id_compose_left. reflexivity.
+simpl. rewrite <- IHh2. simpl. reflexivity.
+simpl. rewrite <- IHh2. simpl. reflexivity.
+simpl. rewrite <- IHh2. simpl. reflexivity.
+simpl. rewrite <- IHh2. simpl. reflexivity.
+simpl. rewrite <- IHh2. simpl. reflexivity.
+simpl. rewrite <- IHh2. simpl. reflexivity.
+simpl. rewrite <- IHh2. simpl. reflexivity.
+
+dependent induction h2.
+rewrite id_fill. rewrite id_compose_left. reflexivity.
+simpl. rewrite <- IHh2. simpl. reflexivity.
+simpl. rewrite <- IHh2. simpl. reflexivity.
+simpl. rewrite <- IHh2. simpl. reflexivity.
+simpl. rewrite <- IHh2. simpl. reflexivity.
+simpl. rewrite <- IHh2. simpl. reflexivity.
+simpl. rewrite <- IHh2. simpl. reflexivity.
+simpl. rewrite <- IHh2. simpl. reflexivity.
+
+dependent induction h2.
+rewrite id_fill. rewrite id_compose_left. reflexivity.
+simpl. rewrite <- IHh2. simpl. reflexivity.
+simpl. rewrite <- IHh2. simpl. reflexivity.
+simpl. rewrite <- IHh2. simpl. reflexivity.
+simpl. rewrite <- IHh2. simpl. reflexivity.
+simpl. rewrite <- IHh2. simpl. reflexivity.
+simpl. rewrite <- IHh2. simpl. reflexivity.
+simpl. rewrite <- IHh2. simpl. reflexivity.
+
+dependent induction h2.
+rewrite id_fill. rewrite id_compose_left. reflexivity.
+simpl. rewrite <- IHh2. simpl. reflexivity.
+simpl. rewrite <- IHh2. simpl. reflexivity.
+simpl. rewrite <- IHh2. simpl. reflexivity.
+simpl. rewrite <- IHh2. simpl. reflexivity.
+simpl. rewrite <- IHh2. simpl. reflexivity.
+simpl. rewrite <- IHh2. simpl. reflexivity.
+simpl. rewrite <- IHh2. simpl. reflexivity.
+Qed.
 
 Inductive item : Type :=
 | item_field : string -> item
@@ -47,17 +194,4 @@ Inductive def : Type :=
 .
 
 Inductive program : Type := Program : list def -> program.
-*)
-
-
-
-
-
-
-
-
-
-
-
-
 
