src/Semantics.v
@@ -1,76 +1,144 @@
+Require Import ch2o.prelude.base.
+Require Import ch2o.prelude.option.
+Require Import Coq.Lists.List.
+Require Import Coq.Program.Equality.
+Require Import Coq.Strings.String.
+
 Require Import Ast.
 Require Import Store.
 Require Import Entities.
 
-Reserved Notation "h1 / f1 / e1 '==>' h2 / f2 / e2"
-  (at level 40, e1 at level 39, h2 at level 39, f1 at level 38, f2 at level 38).
+Reserved Notation "LHS '⇒' RHS" (at level 40).
 
-Inductive step : heap * frame * expr -> heap * frame * expr -> Prop :=
-| E_Seq : forall h f t e,
-    h / f / expr_seq (expr_temp t) e ==> h / f / e
+Open Scope string_scope.
 
-| E_Recover : forall h f t,
-    h / f / expr_recover (expr_temp t) ==> h / f / (expr_temp t)
+Inductive step : heap * list frame * expr -> heap * list frame * expr -> Prop :=
+| E_Seq : forall h f t e stack,
+    (h, f :: stack, expr_seq (expr_temp t) e) ⇒ (h, f :: stack, e)
 
-| E_Local : forall h f t f' name,
-    t = Frame.alloc_temp f ->
-    f' = Frame.set f (TempId t) (Frame.get f (SourceId name)) ->
-    h / f / expr_local name ==> h / f' / expr_temp t
+| E_Recover : forall h f t stack,
+    (h, f :: stack, expr_recover (expr_temp t)) ⇒ (h, f :: stack, (expr_temp t))
 
-| E_Asn_Local : forall h f f' t t' name,
-    t' = Frame.alloc_temp f ->
-    f' = Frame.set (Frame.set f (TempId t') (Frame.get f (SourceId name)))
-              (SourceId name) (Frame.get f (TempId t)) ->
-    h / f / expr_assign_local name (expr_temp t) ==> h / f' / expr_temp t'
+| E_Local : forall h f t f' name stack,
+    not (elem_of t f) ->
+    f' = <[t := f !!! name]> f ->
+    (h, f :: stack, expr_local name) ⇒ (h, f' :: stack, expr_temp t)
 
-| E_Fld : forall h f f' t t' name addr,
-    t' = Frame.alloc_temp f ->
-    v_addr addr = Frame.get f (TempId t) ->
-    f' = Frame.set f (TempId t') (Heap.get_field h addr name) ->
-    h / f / expr_field (expr_temp t) name ==> h / f' / expr_temp t'
+| E_Asn_Local : forall h f f' t t' x stack,
+    not (elem_of t' f) ->
 
-| E_Asn_Field : forall h h' f f' t t' t'' name addr,
-    t'' = Frame.alloc_temp f ->
-    v_addr addr = Frame.get f (TempId t) ->
-    f' = Frame.set f (TempId t'') (Heap.get_field h addr name) ->
-    h' = Heap.set_field h addr name (Frame.get f (TempId t')) ->
+    f' = <[t' := f !!! x]>(<[x := f !!! t]>f) ->
 
-    h / f / expr_assign_field (expr_temp t) name (expr_temp t') ==>
-    h' / f' / expr_temp t''
+    (h, f :: stack, expr_assign_local x (expr_temp t)) ⇒ (h, f' :: stack, expr_temp t')
 
-| E_Seq1 : forall h f f' e1 e1' e2,
-    h / f / e1 ==> h / f' / e1' ->
-    h / f / expr_seq e1 e2 ==> h / f' / expr_seq e1' e2
+| E_Fld : forall h f f' t t' name addr stack,
+    not (elem_of t' f) ->
+    v_addr addr = f !!! t ->
+    f' = <[t' := h !!! (addr, name)]> f ->
+    (h, f :: stack, expr_field (expr_temp t) name) ⇒ (h, f' :: stack, expr_temp t')
 
-| E_Recover1 : forall h f f' e e',
-    h / f / e ==> h / f' / e' ->
-    h / f / expr_recover e ==> h / f' / expr_recover e'
+| E_Asn_Fld : forall h h' f f' t t' t'' name addr stack,
+    not (elem_of t'' f) ->
+    v_addr addr = f !!! t ->
+    f' = <[t'' := h !!! (addr, name)]>f ->
+    h' = <[(addr, name) := f !!! t']>h ->
 
-| E_Asn_Local1 : forall h f f' name e e',
-    h / f / e ==> h / f' / e' ->
-    h / f / expr_assign_local name e ==> h / f' / expr_assign_local name e'
+    (h, f :: stack, expr_assign_field (expr_temp t) name (expr_temp t')) ⇒
+    (h', f' :: stack, expr_temp t'')
 
-| E_Fld1 : forall h f f' e e' name,
-    h / f / e ==> h / f' / e' ->
-    h / f / expr_field e name ==> h / f' / expr_field e' name
+| E_Fld_Null : forall h f t name stack,
+    v_null = f !!! t ->
 
-where "h1 / f1 / e1 '==>' h2 / f2 / e2" := (step (h1,f1,e1) (h2,f2,e2)).
+    (h, f :: stack, expr_field (expr_temp t) name) ⇒
+    (h, f :: stack, expr_temp t)
 
-Reserved Notation "h1 / f1 / e1 '==>*' h2 / f2 / e2"
-  (at level 40, e1 at level 39, h2 at level 39, f1 at level 38, f2 at level 38).
+| E_Asn_Fld_Null : forall h f t t' name stack,
+    v_null = f !!! t ->
 
-Inductive multistep : heap * frame * expr -> heap * frame * expr -> Prop :=
-| multi_refl : forall h f e, multistep (h, f, e) (h, f, e)
+    (h, f :: stack, expr_assign_field (expr_temp t) name (expr_temp t')) ⇒
+    (h, f :: stack, expr_temp t)
 
-| multi_trans : forall h1 f1 e1 h2 f2 e2 h3 f3 e3,
-    h1 / f1 / e1 ==> h2 / f2 / e2 ->
-    h2 / f2 / e2 ==>* h3 / f3 / e3 ->
-    h1 / f1 / e1 ==>* h3 / f3 / e3
-where "h1 / f1 / e1 '==>*' h2 / f2 / e2" := (multistep (h1, f1, e1) (h2, f2, e2)).
+| E_Call_Null : forall h f t name stack,
+    v_null = f !!! t ->
 
-Theorem multi_one : forall h1 f1 e1 h2 f2 e2,
-  h1 / f1 / e1 ==> h2 / f2 / e2 ->
-  h1 / f1 / e1 ==>* h2 / f2 / e2.
+    (h, f :: stack, expr_call (expr_temp t) name) ⇒
+    (h, f :: stack, expr_temp t)
+
+| E_Sync : forall h f f' f'' t hole e0 name stack addr,
+    v_addr addr = f !!! t ->
+
+    f'' = {|
+      method := name;
+      locals := <["this" := (v_addr addr)]>empty;
+      hole := expr_hole_id
+    |} ->
+
+    f' = {|
+      method := f.(method);
+      locals := f.(locals);
+      hole := hole
+    |} ->
+    
+    make_hole e0 (expr_call (expr_temp t) name) hole ->
+
+    (h, f :: stack, e0) ⇒ (h, f'' :: f' :: stack, (expr_local "this"))
+
+| E_Return : forall h f f' f'' hole t t' stack,
+    not (elem_of t' f) ->
+
+    f'' = {|
+      method := f.(method);
+      locals := <[t' := f' !!! t]>f.(locals);
+      hole := expr_hole_id
+    |} ->
+
+    (h, f' :: f :: stack, expr_temp t) ⇒
+    (h, f'' :: stack, fill_hole f.(hole) (expr_temp t'))
+
+| E_Seq1 : forall h h' f f' e1 e1' e2 stack,
+    (h, f :: stack, e1) ⇒ (h', f' :: stack, e1') ->
+    (h, f :: stack, expr_seq e1 e2) ⇒ (h', f' :: stack, expr_seq e1' e2)
+
+| E_Recover1 : forall h h' f f' e e' stack,
+    (h, f :: stack, e) ⇒ (h', f' :: stack, e') ->
+    (h, f :: stack, expr_recover e) ⇒ (h', f' :: stack, expr_recover e')
+
+| E_Asn_Local1 : forall h h' f f' name e e' stack,
+    (h, f :: stack, e) ⇒ (h', f' :: stack, e') ->
+    (h, f :: stack, expr_assign_local name e) ⇒ (h', f' :: stack, expr_assign_local name e')
+
+| E_Fld1 : forall h h' f f' e e' name stack,
+    (h, f :: stack, e) ⇒ (h', f' :: stack, e') ->
+    (h, f :: stack, expr_field e name) ⇒ (h', f' :: stack, expr_field e' name)
+
+| E_Asn_Fld1 : forall h h' f f' e1 e1' e2 name stack,
+    (h, f :: stack, e1) ⇒ (h', f' :: stack, e1') ->
+
+    (h, f :: stack, expr_assign_field e1 name e2) ⇒
+    (h', f' :: stack, expr_assign_field e1' name e2)
+
+| E_Asn_Fld2 : forall h h' f f' t1 e2 e2' name stack,
+    (h, f :: stack, e2) ⇒ (h', f' :: stack, e2') ->
+
+    (h, f :: stack, expr_assign_field (expr_temp t1) name e2) ⇒
+    (h', f' :: stack, expr_assign_field (expr_temp t1) name e2')
+
+where "LHS '⇒' RHS" := (step LHS RHS).
+
+Reserved Notation "LHS '⇒*' RHS" (at level 40).
+
+Inductive multistep : heap * list frame * expr -> heap * list frame * expr -> Prop :=
+| multi_refl : forall h f e, (h, f, e) ⇒* (h, f, e)
+
+| multi_trans : forall h1 f1 e1 h2 f2 e2 h3 f3 e3 stack,
+    (h1, f1::stack, e1) ⇒ (h2, f2::stack, e2) ->
+    (h2, f2::stack, e2) ⇒* (h3, f3::stack, e3) ->
+    (h1, f1::stack, e1) ⇒* (h3, f3::stack, e3)
+where "LHS '⇒*' RHS" := (multistep LHS RHS).
+
+Theorem multi_one : forall h1 f1 e1 h2 f2 e2 stack,
+  (h1, f1 :: stack, e1) ⇒ (h2, f2 :: stack, e2) ->
+  (h1, f1 :: stack, e1) ⇒* (h2, f2 :: stack, e2).
 Proof.
 intros.
 apply multi_trans with (h2 := h2) (f2 := f2) (e2 := e2).
@@ -78,35 +146,93 @@ exact H.
 apply multi_refl.
 Qed.
 
-Theorem multi_concat : forall h1 f1 e1 h2 f2 e2 h3 f3 e3,
-  h1 / f1 / e1 ==>* h2 / f2 / e2 ->
-  h2 / f2 / e2 ==>* h3 / f3 / e3 ->
-  h1 / f1 / e1 ==>* h3 / f3 / e3.
+Theorem multi_concat : forall h1 f1 e1 h2 f2 e2 h3 f3 e3 stack,
+  (h1, f1 :: stack, e1) ⇒* (h2, f2 :: stack, e2) ->
+  (h2, f2 :: stack, e2) ⇒* (h3, f3 :: stack, e3) ->
+  (h1, f1 :: stack, e1) ⇒* (h3, f3 :: stack, e3).
 Proof.
-  intros.
-  generalize dependent h3.
-  generalize dependent f3.
-  generalize dependent e3.
-  induction H.
-  + intros. exact H0.
-  + intros.
-    apply multi_trans with (h2 := h3) (f2 := f3) (e2 := e3).
-    exact H.
-    apply IHmultistep.
-    exact H1.
+intros.
+generalize dependent h3.
+generalize dependent f3.
+generalize dependent e3.
+dependent induction H.
+- intros. exact H0.
+- intros. apply multi_trans with h4 f4 e4.
+  exact H. apply IHmultistep. exact H1.
 Qed.
 
-Lemma E_RecoverN : forall h h' f f' e e',
-    h / f / e ==>* h' / f' / e' ->
-    h / f / expr_recover e ==>* h' / f' / expr_recover e'.
-Admitted.
+Lemma E_RecoverN : forall h h' f f' e e' stack,
+    (h, f :: stack, e) ⇒* (h', f' :: stack, e') ->
+    (h, f :: stack, expr_recover e) ⇒* (h', f' :: stack, expr_recover e').
+Proof.
+intros.
+dependent induction H.
+- apply multi_refl.
+- apply multi_trans with (h2 := h2) (f2 := f2) (e2 := expr_recover e2).
+  apply E_Recover1. exact H.
+  apply IHmultistep.
+Qed.
 
-Lemma E_SeqN : forall h h' f f' e1 e1' e2,
-    h / f / e1 ==>* h' / f' / e1' ->
-    h / f / expr_seq e1 e2 ==>* h' / f' / expr_seq e1' e2.
-Admitted.
+Lemma E_SeqN : forall h h' f f' e1 e1' e2 stack,
+    (h, f :: stack, e1) ⇒* (h', f' :: stack, e1') ->
+    (h, f :: stack, expr_seq e1 e2) ⇒* (h', f' :: stack, expr_seq e1' e2).
+Proof.
+intros.
+dependent induction H.
+- apply multi_refl.
+- apply multi_trans with (h2 := h2) (f2 := f2) (e2 := expr_seq e0 e2).
+  apply E_Seq1. exact H.
+  apply IHmultistep.
+Qed.
 
-Lemma E_Asn_LocalN : forall h h' f f' name e e',
-    h / f / e ==>* h' / f' / e' ->
-    h / f / expr_assign_local name e ==>* h' / f' / expr_assign_local name e'.
-Admitted.
+Lemma E_Asn_LocalN : forall h h' f f' name e e' stack,
+    (h, f :: stack, e) ⇒* (h', f' :: stack, e') ->
+    (h, f :: stack, expr_assign_local name e) ⇒* (h', f' :: stack, expr_assign_local name e').
+Proof.
+intros.
+dependent induction H.
+- apply multi_refl.
+- apply multi_trans with (h2 := h2) (f2 := f2) (e2 := expr_assign_local name e2).
+  apply E_Asn_Local1. exact H.
+  apply IHmultistep.
+Qed.
+
+Lemma E_FldN : forall h h' f f' e e' name stack,
+    (h, f :: stack, e) ⇒* (h', f' :: stack, e') ->
+    (h, f :: stack, expr_field e name) ⇒* (h', f' :: stack, expr_field e' name).
+Proof.
+intros.
+dependent induction H.
+- apply multi_refl.
+- apply multi_trans with (h2 := h2) (f2 := f2) (e2 := expr_field e2 name).
+  apply E_Fld1. exact H.
+  apply IHmultistep.
+Qed.
+
+Lemma E_Asn_Fld1N : forall h h' f f' e1 e1' e2 name stack,
+    (h, f :: stack, e1) ⇒* (h', f' :: stack, e1') ->
+
+    (h, f :: stack, expr_assign_field e1 name e2) ⇒*
+    (h', f' :: stack, expr_assign_field e1' name e2).
+Proof.
+intros.
+dependent induction H.
+apply multi_refl.
+- apply multi_trans with (h2 := h2) (f2 := f2) (e2 := expr_assign_field e0 name e2).
+  apply E_Asn_Fld1. exact H.
+  apply IHmultistep.
+Qed.
+
+Lemma E_Asn_Fld2N : forall h h' f f' t1 e2 e2' name stack,
+    (h, f :: stack, e2) ⇒* (h', f' :: stack, e2') ->
+
+    (h, f :: stack, expr_assign_field (expr_temp t1) name e2) ⇒*
+    (h', f' :: stack, expr_assign_field (expr_temp t1) name e2').
+Proof.
+intros.
+dependent induction H.
+apply multi_refl.
+- apply multi_trans with (h2 := h2) (f2 := f2) (e2 := expr_assign_field (expr_temp t1) name e0).
+  apply E_Asn_Fld2. exact H.
+  apply IHmultistep.
+Qed.
