src/Eval.v
@@ -8,127 +8,97 @@ Require Import Coq.Strings.String.
 Require Import Coq.Structures.Equalities.
 Require Import Coq.Arith.EqNat.
 
+Require Import ch2o.prelude.base.
+
 Require Import Ast.
 Require Import Semantics.
 Require Import Entities.
 Require Import Store.
 
-Fixpoint eval (h: heap) (f: frame) (e: expr) : heap * frame * nat :=
-  match e with
-  | expr_temp t => (h, f, t)
+Fixpoint eval' (h: heap) (stack: list frame) (e: expr) (cps: expr_hole) : option (heap * list frame * expr) :=
+  match stack, e with
+  | nil, _ => None
+  | (_ :: nil), expr_temp t => None
 
-  | expr_recover e' => eval h f e'
-  | expr_local name =>
-      let t := Frame.alloc_temp f in
-      let f' := Frame.set f (TempId t) (Frame.get f (SourceId name)) in
-      (h, f', t)
+  | (f :: f' :: stack'), expr_temp t =>
+    let cps := f'.(hole) in
+    let t' := fresh f' in
+    let value := f !!! t in
+    let f'' := {|
+      method := f'.(method);
+      locals := <[t' := value]>f'.(locals);
+      hole := expr_hole_id
+    |} in
+    Some (h, f'' :: stack', fill_hole cps (expr_temp t'))
 
-  | expr_assign_local name e =>
-      let '(h', f', t) := eval h f e in
-      let t' := Frame.alloc_temp f' in
-      let f'' := Frame.set f' (TempId t') (Frame.get f' (SourceId name)) in
-      let f''' := Frame.set f'' (SourceId name) (Frame.get f' (TempId t)) in
-      (h', f''', t')
+  | (f :: stack'), expr_call (expr_temp t) name =>
+    match f !!! t with
+    | v_addr addr => 
+      let f'' := {|
+        method := name;
+        locals := <["this" := v_addr addr]>empty;
+        hole := expr_hole_id
+      |} in
 
-  | expr_field e name =>
-      let '(h', f', t) := eval h f e in
-      match Frame.get f' (TempId t) with
-      | v_addr addr =>
-        let t' := Frame.alloc_temp f' in
-        let value := Heap.get_field h' addr name in
-        let f'' := Frame.set f' (TempId t') value in
+      let f' := {|
+        method := f.(method);
+        locals := f.(locals);
+        hole := cps
+      |} in
 
-        (h', f'', t')
-      | v_null => (h', f', t)
-      end
+      Some (h, f'' :: f' :: stack', expr_local "this")
 
-  | expr_assign_field e name e' =>
-      let '(h', f', t) := eval h f e in
-      let '(h'', f'', t') := eval h' f' e' in
+    | v_null => Some (h, f :: stack', fill_hole cps (expr_temp t))
+    end
 
-      match Frame.get f'' (TempId t) with
-      | v_addr addr =>
-        let t''' := Frame.alloc_temp f'' in
-        let old_value := Heap.get_field h'' addr name in
-        let value := Frame.get f'' (TempId t') in
+  | (f :: stack'), expr_seq (expr_temp t) e' => Some (h, f :: stack', fill_hole cps e')
 
-        let h''' := Heap.set_field h'' addr name value in
-        let f''' := Frame.set f'' (TempId t''') old_value in
+  | (f :: stack'), expr_recover (expr_temp t) => Some (h, f :: stack', fill_hole cps (expr_temp t))
 
-        (h''', f''', t''')
-      | v_null => (h'', f'', t)
-      end
+  | (f :: stack'), expr_local name =>
+      let t := fresh f in
+      let f' := <[t := f !!! name]>f in
 
-  | expr_seq e1 e2 =>
-      let '(h', f', _) := eval h f e1
-      in eval h' f' e2
+      Some (h, f' :: stack', fill_hole cps (expr_temp t))
+
+  | (f :: stack'), expr_assign_local name (expr_temp t) =>
+      let t' := fresh f in
+      let f' := <[t' := f !!! name]>(<[name := f !!! t]>f) in
+
+      Some (h, f' :: stack', fill_hole cps (expr_temp t'))
+
+  | (f :: stack'), expr_field (expr_temp t) name =>
+    match f !!! t with
+    | v_addr addr => 
+      let t' := fresh f in
+      let f' := <[t' := h !!! (addr, name)]>f in
+
+      Some (h, f' :: stack', fill_hole cps (expr_temp t'))
+
+    | v_null => Some (h, f :: stack', fill_hole cps (expr_temp t))
+    end
+
+  | (f :: stack'), expr_assign_field (expr_temp t) name (expr_temp t') =>
+    match f !!! t with
+    | v_addr addr => 
+      let t'' := fresh f in
+      let f' := <[t'' := h !!! (addr, name)]>f in
+      let h' := <[(addr, name) := f !!! t']>h in
+
+      Some (h', f' :: stack', fill_hole cps (expr_temp t''))
+
+    | v_null => Some (h, f :: stack', fill_hole cps (expr_temp t))
+    end
+
+  | stack, expr_seq e1 e2 => eval' h stack e1 (compose_hole cps (expr_hole_seq expr_hole_id e2))
+  | stack, expr_recover e1 => eval' h stack e1 (compose_hole cps (expr_hole_recover expr_hole_id))
+
+  | stack, expr_assign_local name e1 => eval' h stack e1 (compose_hole cps (expr_hole_assign_local name expr_hole_id))
+  | stack, expr_field e1 name => eval' h stack e1 (compose_hole cps (expr_hole_field expr_hole_id name))
+  | stack, expr_assign_field e1 name (expr_temp t2) => eval' h stack e1 (compose_hole cps (expr_hole_assign_field2 expr_hole_id name t2))
+  | stack, expr_assign_field e1 name e2 => eval' h stack e2 (compose_hole cps (expr_hole_assign_field1 e1 name expr_hole_id))
+  | stack, expr_call e1 name => eval' h stack e1 (compose_hole cps (expr_hole_call1 expr_hole_id name))
   end.
 
-Theorem eval_step: forall h h' f f' e t,
-  (eval h f e = (h', f', t) -> h / f / e ==>* h' / f' / expr_temp t).
-Admitted.
-
-(*
-Proof.
-intros f e.
-generalize dependent f.
-induction e.
-+ intros.
-  simpl in H.
-  inversion H.
-  symmetry in H1.
-  symmetry in H2.
-  rewrite H1.
-  rewrite H2.
-  apply multi_refl.
-
-+ intros.
-  simpl in H.
-  remember (eval f e1) as E.
-  symmetry in HeqE.
-  destruct E.
-
-  apply multi_concat with (f2 := f0) (e2 := (expr_seq (expr_temp n) e2)).
-  - apply E_SeqN.
-    apply IHe1.
-    exact HeqE.
-  - apply multi_trans with (f2 := f0) (e2 := e2).
-    * apply E_Seq.
-    * apply IHe2.
-      exact H.
-
-+ intros.
-  simpl in H.
-  apply multi_concat with (f2 := f') (e2 := expr_recover (expr_temp t)).
-  - apply E_RecoverN.
-    apply IHe.
-    exact H.
-  - apply multi_one.
-    apply E_Recover.
-
-+ intros.
-  simpl in H.
-  inversion H.
-  apply multi_one.
-  apply E_Local.
-  reflexivity.
-  reflexivity.
-
-+ intros.
-  simpl in H.
-  remember (eval f e) as E.
-  symmetry in HeqE.
-  destruct E.
-  apply multi_concat with (f2 := f0) (e2 := expr_assign_local s (expr_temp n)).
-  - apply E_Asn_LocalN.
-    apply IHe.
-    exact HeqE.
-
-  - apply multi_one.
-    inversion H.
-    apply E_Asn_Local.
-    * reflexivity.
-    * reflexivity.
-
-Qed.
-*)
+Definition eval (h: heap) (stack: list frame) (e: expr) : option (heap * list frame * expr) :=
+  eval' h stack e expr_hole_id.
