src/Extract.v
@@ -1,22 +1,31 @@
 Require Import Eval.
+Require Import Ast.
 Require Import Semantics.
 Require Import Entities.
+Require Import ch2o.prelude.base.
+Require Import ch2o.prelude.stringmap.
+Require Import ch2o.prelude.nmap.
 
+Require Import Coq.Lists.List.
 Require Import Coq.Strings.String.
 Require Import Coq.extraction.ExtrHaskellBasic.
 Require Import Coq.extraction.ExtrHaskellString.
 Require Import Coq.extraction.ExtrHaskellNatInteger.
 
-Definition init : heap * frame :=
-    let h := Heap.empty in
-    let f := Frame.empty in
+Definition init : heap * list frame :=
+    let obj := {| name := "Foo"; fields := empty |} in
+    let h := empty in
+    let addr : N := Nfresh h in
+    let h' := <[ addr := obj ]>h in
+    let f := {|
+      method := "<init>";
+      locals := <[ "x" := v_addr addr ]>empty;
+      hole := expr_hole_id
+    |} in
 
-    let (h', addr) := Heap.create h "Foo" in
-    let f' := Frame.set f (SourceId "x") (v_addr addr) in
-
-    (h', f').
+    (h', f::nil).
 
 Extraction Language Haskell.
-Cd "out".
-Separate Extraction init eval.
-Cd "..".
+Extraction "main/Extracted.pre.hs"
+    init eval frame local_id.
+
