SConstruct
@@ -1,0 +1,33 @@
+# Copyright (c) 2012-2015, Robbert Krebbers.
+# This file is distributed under the terms of the BSD license.
+import os, glob, string
+import subprocess
+
+modules = ["ch2o/prelude", "src"]
+
+Rs = '-R ch2o ch2o -R src pony'
+env = DefaultEnvironment(ENV = os.environ,tools=['default', 'Coq'], COQFLAGS=Rs)
+
+# Coq dependencies
+vs = [x for m in modules for x in glob.glob(m + '/*.v')]
+if os.system('coqdep ' + Rs + ' ' + ' '.join(map(str, vs)) + ' > deps'): Exit(2)
+ParseDepends('deps')
+
+
+def add_qualified(target, source, env):
+  subprocess.check_call(['sed', '-e', 's/module .* where/module Extracted where/',
+                         '-e', '/^module/a\\\nimport qualified Data.Bits',
+                         '-e', '/^module/a\\\nimport qualified Data.Char'],
+                        stdin=open(str(source[0])),
+                        stdout=open(str(target[0]), 'w'))
+
+# Coq files
+for v in vs:
+  env.Coq(v)
+
+env.Depends('main/Extracted.pre.hs', 'src/Extract.vo')
+
+env.Command('main/Extracted.hs',
+            'main/Extracted.pre.hs',
+            Action(add_qualified))
+
